<?xml version="1.0" encoding="UTF-8"?>

<section xml:id="s_deMoivre" xmlns:xi="http://www.w3.org/2001/XInclude">
    <title>De Moivre's formula</title>
<introduction>
    <p>
        The polar form description of complex multiplication given in <xref ref="th_polar_form"/> leads naturally to a similar description of integer powers of complex numbers, called <em>de Moivre's formula</em>. 
    </p>
</introduction>
<subsection xml:id="ss_deMoivre">
    <title>De Moivre's formula</title>
    
<theorem xml:id="th_deMoivre">
    <title>De Moivre's formula</title>
    <statement>
        <p>
            Let <m>z=r(\cos\theta+i\sin\theta)</m>, where <m>r\geq 0</m> and <m>\theta\in \R</m>. 
            <ol>
                <li>
                    <title>Nonnegative integer powers</title>
                    <p>
                       For all nonnegative integers <m>n</m>, we have 
                <men xml:id="eq_deMoivres">
                z^n=r^n(\cos(n\theta)+i\sin(n\theta))
                </men>. 
                    </p>
                </li>
                <li>
                    <title>Negative integer powers</title>
                    <p>
                        Assume <m>z\ne 0</m>. For all positive integers <m>n</m> we have 
            <men xml:id="eq_deMoivres_neg">
                z^{-n}=r^{-n}(\cos(-n\theta)+i\sin(-n\theta))
            </men>.
                    </p>
                </li>
            </ol>
        </p>
    </statement>
    <proof>
        <p>
            First observe that statement (2) follows from (1) since for <m>z\ne 0</m> and positive integer <m>n</m> we have 
            <md>
                <mrow>z^{-n} \amp= (z^{-1})^n </mrow>
                <mrow> \amp = (r^{-1}(\cos(-\theta)+i\sin(-\theta))^n \amp (<xref ref="th_polar_mult" text="global"/>)</mrow>
                <mrow> \amp = (r^{-1})^n(\cos(-n\theta)+i\sin(-n\theta))</mrow>
                <mrow> \amp = r^{-n}(\cos(-n\theta)+i\sin(-n\theta)) \amp \text{(by (1))}</mrow>
            </md>.
        </p>
        <p>
            The proof of (1) is by induction on <m>n\geq 0</m>. (See <xref ref="ss_mathematical_induction" text="title"/>.)
        </p>
        <p>
            Base case: <m>n=0</m>. We have 
            <md>
                <mrow>r^0(\cos (0\theta)+i\sin(0\theta)) \amp = 1(\cos 0+i\sin 0) </mrow>
                <mrow> \amp = 1</mrow>
                <mrow> \amp = z^0 \amp (<xref ref="d_integer_powers" text="global"/>)</mrow>
            </md>,
            as desired.
        </p>
        <p>
            Induction step: we assume the statement is true for <m>n</m>, and show it is true for <m>n+1</m>. Thus we assume that 
            <me>
                z^n=r^n(\cos(n\theta)+i\sin(n\theta))
            </me>.
            It follows that 
            <md>
                <mrow>z^{n+1} \amp = z\, z^n</mrow>
                <mrow> \amp = z\cdot r^n(\cos(n\theta)+i\sin(n\theta)) \amp (\text{ind. hyp.})</mrow>
                <mrow> \amp = r(\cos \theta+i\sin\theta)\cdot r^n(\cos(n\theta)+i\sin(n\theta)) </mrow>
                <mrow> \amp = r\, r^{n+1}(\cos(\theta+n\theta)+i\sin(\theta+n\theta)) \amp \text{(polar mult.)}</mrow>
                <mrow> \amp =r^{n+1}(\cos((n+1)\theta)+i\sin((n+1)\theta))</mrow>
            </md>,
            as desired.
        </p>
    </proof>
</theorem>
<example xml:id="eg_deMoivre">
<title>De Moivre's formula</title>
<statement>
<p>
Compute <m>(1+i)^{14}</m>. Express you answer in both polar form and in the form <m>a+ib</m>.   
</p>
</statement>
<solution>
<p>
First write <m>1+i</m> in polar form as <m>1+i=\sqrt{2}(\cos \pi/4+i\sin\pi/4)</m>. Using de Moivre's formula, we have 
<md>
    <mrow>(1+i)^{14} \amp = (\sqrt{2})^{14}(\cos (14\pi/4)+i\sin(14\pi/ 4))</mrow>
    <mrow> \amp = 2^{14/2}(\cos 7\pi/2+i\sin 7\pi/2) \amp (\sqrt{2}=2^{1/2})</mrow>
    <mrow> \amp 128(0-i) \amp (7\pi/2=3\pi/2+2\pi)</mrow>
    <mrow> \amp =-128i</mrow>
</md>.
</p>
</solution>
</example>
<example xml:id="eg_deMoivre_trig">
<title>Double-angle formulas</title>
<statement>
<p>
Use de Moivre's formula to prove the double-angle formulas:
<md>
    <mrow>\cos 2\theta \amp =\cos^2\theta-\sin^2\theta</mrow>
    <mrow>\sin 2\theta \amp = 2\sin\theta\cos\theta</mrow>
</md>.
</p>
</statement>
<solution>
<p>
Let <m>z=\cos\theta+i\sin\theta</m>. We may compute <m>z^2=z\, z</m> using the algebraic definition of complex multiplication, or by using de Moivre's formula. Equating the two resulting expressions yields 
<me>
    \cos 2\theta+i\sin 2\theta =\cos^2\theta-\sin^2\theta+ 2\sin\theta\cos\theta i
</me>.
From the definition of complex number equality, it follows that 
<md>
    <mrow>\cos 2\theta \amp =\cos^2\theta-\sin^2\theta</mrow>
    <mrow>\sin 2\theta \amp = 2\sin\theta\cos\theta</mrow>
</md>,
as desired.
</p>
</solution>
</example>
<example xml:id="eg_deMoivre_triple">
<title>Triple-angle formula</title>
<statement>
<p>
Use de Moivre's formula to derive triple-angle formulas for <m>\cos\theta</m> and <m>\sin\theta</m>. In more detail, find polynomials <m>f(x,y)</m> and <m>g(x,y)</m> such that 
<md>
    <mrow>\cos 3\theta \amp = f(\cos\theta,\sin\theta)</mrow>
    <mrow>\sin 3\theta \amp = g(\cos\theta,\sin\theta)</mrow>
</md>.
You may use the fact that the binomial theorem holds for complex numbers: <ie/>, given any <m>z,w\in \C</m> and positive integer <m>n</m>, we have 
<me>
    (z+w)^n=\sum_{k=0}^n {n \choose k} z^{n-k}w^k=z^n+{n\choose 1} z^{n-1}w+\cdots +{n \choose n-1}zw^{n-1}+w^n
</me>,
where 
<me>
    {n\choose k}=\frac{n!}{k!\, (n-k)!}
</me>.
</p>
</statement>
<solution>
<p>
Let as an exercise. 
</p>
</solution>
</example>

</subsection>
<subsection xml:id="ss_nth_roots">
    <title><m>n</m>-th roots</title>
<p>
    One powerful application of de Moivre's formula is that it allows us to compute all <m>n</m>-th roots of a given complex number <m>w</m>. 
</p>
<definition xml:id="d_nth_root">
<title><m>n</m>-th roots</title>
<statement>
<p>
Let <m>n</m> be a positive integer and let <m>w\in \C</m>. An <term><m>n</m>-th root</term> of <m>w</m> is a complex number <m>z\in \C</m> satisfying <m>z^n=w</m>. Equivalently, an <m>n</m>-th root of <m>w</m> is a complex root (or zero) of the polynomial 
<me>
    f(z)=z^n - w
</me>.
An <term><m>n</m>-th root of unity</term> is an <m>n</m>-th root of <m>1</m>. 
</p>
</statement>
</definition>
<example xml:id="eg_3d_root">
<title>Cube-roots of <m>8i</m></title>
<statement>
<p>
Find all cube-roots of <m>8i</m> and sketch these as points in the complex plane. You may express your answer in polar form. 
</p>
</statement>
<solution>
<p>
First write <m>8i</m> in polar form as <m>8i=8(\cos \pi/2+i\sin \pi/2)</m>. If <m>z=r(\cos\theta+i\sin\theta)</m> satisfies <m>z^3=8i</m>, then using de Moivre's theorem we would have 
<me>
    r^3(\cos 3\theta+i\sin 3\theta)=8(\cos \pi/2+i\sin \pi/2)
</me>.
Using <xref ref="th_polar_form"/> we conclude that we must have 
<md>
    <mrow>r^3 \amp =8</mrow>
    <mrow>3\theta \amp =\pi/2+2\pi k \text{ for some } k\in \Z</mrow>
</md>,
or equivalently, 
<md>
    <mrow>r \amp =2</mrow>
    <mrow>\theta \amp = \pi/6+2\pi k/3 \text{ for some } k\in \Z </mrow>
</md>.
Taking <m>k=0,1,2</m>, we see that 
<md>
    <mrow>z_0 \amp = 2(\cos(\pi/6)+i\sin(\pi/6))=\sqrt{3}+i</mrow>
    <mrow>z_1 \amp = 2(\cos(5\pi/6)+i\sin(5\pi/6))=-\sqrt{3}+i</mrow>
    <mrow>z_2 \amp = 2(\cos(3\pi/2)+i\sin(3\pi/2))=-2i</mrow>
</md>
are cube-roots of <m>8i</m>. We claim further that these are all of the cube-roots of <m>8i</m>. This follows from the fact that any angle of the form <m>\pi/6+2\pi k/n</m> is obtained from one of the three angles <m>pi/6, 5\pi/6, 3\pi/2</m> by adding a multiple of <m>2\pi</m>. 
</p>
<figure xml:id="fig_cuberoots_8i">
    <caption>Cube-roots of <m>8i</m></caption>
    <image width="100%">
        <shortdescription>Cube-roots of 8i</shortdescription>
        <sageplot>
S=circle((0,0),2,color="blue", ticks=[list(range(-2,3)),list(range(-2,3))],ymin=-2)
p=vector((2*cos(pi/6),2*sin(pi/6)))
q=vector((2*cos(5*pi/6),2*sin(5*pi/6)))
r=vector((0,-2))
P=point(p,color="red", size=70)
Q=point(q,color="red", size=70)
R=point(r,color="red", size=70)
l1=line(((0,0),p),color="red",linestyle="dashed")
l2=line(((0,0),q),color="red",linestyle="dashed")
l3=line(((0,0),r),color="red",linestyle="dashed", thickness=2)
t1=text("$z_0=2(\\cos(\\pi/6)+i\\sin(\\pi/6))$", 1.1*p, color="black", fontsize=16, horizontal_alignment="left")
t2=text("$z_1=2(\\cos(5\\pi/6)+i\\sin(5\\pi/6))$", 1.1*q, color="black", fontsize=16, horizontal_alignment="right")
t3=text("$z_2=-2i$", 1.2*r, color="black", fontsize=16, horizontal_alignment="center")
l1+l2+l3+S+P+Q+R+t1+t2+t3
        </sageplot>
    </image>
</figure>
</solution>
</example>
<p>
    The reasoning in <xref ref="eg_3d_root"/> can easily be generalized to produce a procedure for computing <m>n</m>-th roots of an arbitrary complex number. 
</p>
<theorem xml:id="th_nth_roots">
    <title><m>n</m>-th roots</title>
    <statement>
        <p>
            Let <m>n</m> be a positive integer. A nonzero complex number <m>w</m> has <m>n</m> distinct <m>n</m>-th roots. In more detail, writing <m>w</m> in polar form as <m>w=r(\cos\theta+i\sin\theta)</m>, the <m>n</m>-th roots of <m>w</m> are <m>z_0,z_1,\dots, z_{n-1}</m>, where for all <m>0\leq k\leq n-1</m>, we have 
            <men xml:id="eq_nth_roots">
                z_k=\sqrt[n]{r}(\cos(\theta/n+2\pi k/n)+i\sin(\theta/n+2\pi k/n))
            </men>.
        </p>
    </statement>
    <proof>
        <p>
            We seek <m>z=s(\cos\psi+i\sin\psi)</m> (<m>s\geq 0</m>, <m>\psi\in \R</m>) satisfying <m>z^n=w</m>. By de Moivre's formula, this is equivalent to 
            <me>
                s^n(\cos(n\psi)+i\sin(n\psi))=r(\cos\theta+i\sin\theta)
            </me>.
            By <xref ref="th_polar_form"/>, this is true if and only if 
            <md>
                <mrow>s^n \amp = r</mrow>
                <mrow>n\psi \amp = \theta+2\pi k \text{ for some } k\in \Z</mrow>
            </md>.
            Solving for <m>s</m> and <m>\psi</m> we conclude that 
            <md>
                <mrow>s \amp = \sqrt[n]{r}</mrow>
                <mrow>\psi \amp = \theta/n +2\pi k/n \text{ for some } k\in \Z</mrow>
            </md>.
            It follows that the complex numbers 
            <me>
                z_k=\sqrt[n]{r}(\cos(\theta/n+2\pi k/n)+i\sin(\theta/n+2\pi k/n)), 0\leq k\leq n-1
            </me>
            are <m>n</m>-th roots of <m>w</m>. That they are <em>distinct</em> follows again from <xref ref="th_polar_form"/> and the fact that  
            <me>
               (\theta/n+2\pi k/n)-(\theta/n+2\pi j/n) = 2\pi(k-j)/n &lt; 2\pi
            </me>
            for all <m>0\leq j&lt; k\leq n-1</m>.  Lastly, since the polynomial <m>f(z)=z^n-w</m> has <em>at most</em> <m>n</m> distinct roots (see <xref ref="th_poly_elem"/>), the <m>n</m> roots <m>z_k</m> are the only <m>n</m>-th roots of <m>w</m>.   
        </p>
    </proof>
</theorem>
<remark>
<title>Visualizing <m>n</m>-th roots</title>
<p>
Let <m>z_0, z_1, \dots, z_{n-1}</m> be the distinct <m>n</m>-th roots of the nonzero complex number <m>w</m>, as described in <xref ref="eq_nth_roots"/>. We make some geometric observations about the <m>z_k</m>: 
<ul>
    <li>
        <p>
            Each <m>z_k</m> has modulus <m>\sqrt[n]{r}</m>, and thus lives on the circle of radius <m>\sqrt[n]{r}</m> centered at the origin. 
        </p>
    </li>
    <li>
        <p>
            Looking at the arguments of the <m>z_k</m>, we see that for each <m>k\geq 1</m>, <m>z_k</m> is obtained from <m>z_{k-1}</m> by a rotation of <m>2\pi/n</m> about the origin. It follows that starting with <m>z_0</m>, we can obtain the other roots by successive rotation by <m>2\pi/n</m>.  
        </p>
    </li>
    <li>
        <p>
            From the previous observations, it follows that the <m>n</m> distinct <m>n</m>-th roots of <m>w</m> are the vertices of a regular <m>n</m>-gon inscribed in the circle of radius <m>\sqrt[n]{r}</m> centered at the origin. (See <xref ref="fig_cuberoots_8i"/>.)
        </p>
    </li>
</ul>
</p>
</remark>

</subsection>
<subsection xml:id="ss_polynomials">
    <title>Polynomials</title>
   <p>
    We can view formula <xref ref="eq_nth_roots"/> as providing explicit roots to the polynomial <m>f(z)=z^n-w</m>, which in turn allows us to factor <m>f</m> into linear terms. To make proper sense of this, we  introduce some terminology and elementary facts around complex polynomials.
   </p> 
   <definition xml:id="d_polynomials">
   <title>Polynomials</title>
     <statement>
    <p>
      A <term>(complex) polynomial</term> is a function <m>f\colon \C\rightarrow \C</m> of the form 
      <men xml:id="eq_poly">
      f(z)=a_nz^n+a_{n-1}z^{n-1}+\cdots +a_1z+a_0
      </men>,
      where <m>n</m> is a nonnegative integer and <m>a_k\in \C</m> for all <m>0\leq k\leq n</m>. 
      </p>
      <p>
        We call <m>a_kx^k</m> the <m>k</m>-th <term>term</term> of <m>f</m>, and <m>a_k</m> the <m>k</m>-th <term>coefficient</term>; <m>a_0</m> is called the <term>constant term</term> of <m>f</m>. 
    </p>
    <p>If <m>a_n\ne 0</m>, then <m>a_nx^{n}</m> is called the <term>leading term</term> of <m>f</m>, <m>a_{n}</m>
      its <term>leading coefficient</term>, and <m>n</m> the <term>degree</term>, denoted <m>\deg f=n</m>. 
      </p>
      <p>
        Lastly, a <term>root</term> (or <term>zero</term>) of <m>f</m> is a a complex number <m>w</m> satisfying  <m>f(w)=0</m>. 
      </p>
  </statement>
</definition>
<theorem xml:id="th_poly_elem">
  <title>Elementary properties of polynomials</title>
  <statement>
      <p>
        <ol>
        <li>
        <p>
          If <m>f</m> and <m>g</m> are polynomials, then so are <m>f+g</m>, <m>fg</m>, and <m>cf</m> for any <m>c\in \C</m>. 
        </p>
      </li>
      <li>
        <p>
          If <m>f</m> is a polynomial  and <m>w_0\in \C</m> is a root of <m>f</m>, then there is a polynomial <m>g</m> such that
          <men xml:id="eq_poly_factor">
            f(z)=(z-w_0)g(z)
          </men>.
        </p>
      </li>
      <li xml:id="th_at_most_n_roots">
        <p>
          If <m>f</m> is a polynomial of degree <m>n</m>, then <m>f</m> has at most <m>n</m> distinct roots.
        </p>
      </li>
    </ol>
    </p>
  </statement>
</theorem>
<p>
    Given a nonzero <m>w\in \C</m> and positive integer <m>n</m>, let <m>z_0,z_1,\dots, z_{n-1}</m> be the <m>n</m> distinct <m>n</m>-th roots of <m>w</m>. Since <m>z_k</m> is a root of <m>f(z)=z^n-w</m> for all <m>0\leq k\leq n-1</m>, it follows that we can factor <m>f</m> into linear factors as 
    <me>
       f(z)=z^n-w =(z-w_0)(z-w_1)\cdots (z-w_{n-1})
    </me>.
    In particular, we now know how to completely factor any <em>real</em> polynomial of the form <m>f(z)=z^n-a</m>, where <m>a\in \R</m>. The next theorem delves into factorization details of the polynomial <m>f(z)=z^n-1</m>.  
</p>
<theorem xml:id="th_roots_unity">
    <title>Roots of unity</title>
    <statement>
        <p>
            Fix a positive integer <m>n</m> and let <m>f(z)=z^n-1</m>.
        <ol>
            <li>
                <p>
                    The <m>n</m> distinct roots of <m>f</m> are 
                    <me>
                        \zeta_k=\cos(2\pi k/n)+i\sin(2\pi k/n)
                    </me>,
                    where <m>0\leq k\leq n-1</m>. Note that <m>\zeta_0=1</m>.
                </p>
            </li>
            <li>
                <p>
                    <m>f(z)</m> factors as 
                    <mdn>
                        <mrow xml:id="eq_cyclo_split">z^n-1\amp=\prod_{k=0}^{n-1}(z-\zeta_k) </mrow>
                        <mrow> \amp =(z-1)\prod_{k=1}^{n-1}(z-\zeta_k)</mrow>
                    </mdn>.
                </p>
            </li>
            <li>
                <p>
                    We have 
                    <men xml:id="eq_cyclo_factor">z^n-1=(z-1)(z^{n-1}+z^{n-2}+\cdots +z+1)
                    </men>
                    and thus, letting <m>g(z)=z^{n-1}+z^{n-2}+\cdots +z+1</m>, 
                    <me>
                        g(z)=\prod_{k=1}^{n-1}(z-\zeta_k)
                    </me>.
                </p>
            </li>
        </ol>
        </p>
    </statement>
</theorem>
<example xml:id="eg_factor_sextic">
<title>Factoring <m>f(x)=x^6-1</m> </title>
<statement>
<p>
Give two distinct factorizations of <m>f(x)=x^6-1</m>:
<ol>
    <li>
        <p>
            as a product of irreducible real polynomials;
        </p>
    </li>
    <li>
        <p>
            as a product of linear terms with complex coefficients.
        </p>
    </li>
</ol>
</p>
</statement>
<solution>
<p>
<ol>
    <li>
        <p>
            Using the difference of squares factoring identity, we have 
            <me>
                x^6-1=(x^3-1)(x^3+1)
            </me>.
            Next, since <m>1</m> is a root of <m>x^3-1</m>, and <m>-1</m> is a root of <m>x^3+1</m>, we can use polynomial division to factor 
            <md>
                <mrow>x^3-1 \amp = (x-1)(x^2+x+1) \amp (x^3+1)\amp=(x+1)(x^2-x+1)</mrow>
            </md>.
            It is now easy to see, using the quadratic formula, that <m>x^2+x+1</m> and <m>x^2-x+1</m> are irreducible over <m>\R</m>, since they have no real roots. Thus 
            <me>
                x^6-1=(x-1)(x+1)(x^2+x+1)(x^2-x-1)
            </me>
            is a factorization of <m>x^6-1</m> into irreducible real polynomials. 
        </p>
    </li>
    <li>
        <p>
            Using <xref ref="th_roots_unity"/>, we have 
            <md>
                <mrow>x^6-1 \amp =\prod_{k=0}^{5}(x-\zeta_k)</mrow>
            </md>,
            where 
            <me>
                \zeta_k=\cos(2\pi k/6+i\sin 2\pi k /6)=\cos(\pi k/3)+i\sin(\pi k/3)
            </me>.
        </p>
    </li>
</ol>
</p>
</solution>
</example>

<p>
    Take a moment to survey these results: thanks to complex numbers, we now know how to completely factor the following polynomials:
    <md>
        <mrow>f(z) \amp = z^n-w \amp </mrow>
        <mrow> f(z)\amp =z^n-1  </mrow>
        <mrow>f(z)\amp =z^{n-1}+z^{n-2}+\cdots +z+1 </mrow>
    </md>.
    Pretty impressive! As it turns out, every complex polynomial can be factored in this manner. This is the content of the <em>fundamental theorem of algebra</em>, a full proof of which we will be able to provide by the end of this course. 
</p>
<theorem xml:id="th_fund_alg">
    <title>Fundamental theorem of algebra</title>
    <statement>
    <p>
    Let <m>f\colon \C\rightarrow \C</m> be a nonconstant polynomial: <ie/>, <m>\deg f \geq 1</m>. 
    <ol>
        <li>
            <title><m>f</m> has a complex root</title>
            <p>
                There is a <m>w\in \C</m> such that  <m>f(w)=0</m>. 
            </p>
        </li>
        <li>
            <title><m>f</m> spits completely</title>
            <p>
                There are complex numbers <m>w_1,w_2,\dots, w_n</m> such that 
                <me>
                    f(z)=c\prod_{k=1}^n(z-w_k)
                </me>.
            </p>
        </li>
    </ol>
    </p>
    </statement>
</theorem>

</subsection>



    

</section>