<?xml version="1.0" encoding="UTF-8"?>

<section xml:id="s_laurent_series" xmlns:xi="http://www.w3.org/2001/XInclude">
    <title>Laurent series</title>
    <p>
        We have begun to see the utility of power series representations for functions <m>f</m> that are holomorphic on an open ball <m>B_R(z_0)</m>. It turns out that much of this theory (and its attendant benefits) can be extended to more general functions by relaxing somewhat the differentiability condition. Namely, we will develop a series representation for functions <m>f</m> which are holomorphic not on a full open ball centered at <m>z_0</m>, but only on an annulus of the form <m>\{z\in \C\colon R_1&lt; \abs{z-z_0}&lt; R_2\}</m>. We proceed directly to <xref ref="th_laurent"/>, which will serve to motivate our study of <em>Laurent series</em>. 
    </p>
    <theorem xml:id="th_laurent">
    <title>Laurent's theorem</title>
    <statement>
    <p>
    Let <m>z_0\in \C</m> and <m>A=\{z\colon R_1&lt; \abs{z-z_0} &lt; R_2\}</m>, where <m>R_1, R_2\in \C\cup \{\infty\}</m> and <m>0\leq R_1&lt; R_2</m>. If <m>f</m> is holomorphic on <m>A</m>, then there are power series 
    <md>
        <mrow>g(u) \amp =\sum_{n=0}^\infty a_nu^n
        \amp h(u) \amp =\sum_{m=1}^\infty b_mu^m</mrow>
    </md>
    such that 
    <md>
      <mrow>f(z) \amp = g(z-z_0)+h(1/(z-z_0))</mrow>
      <mrow> \amp =  \cdots +\frac{b_2}{(z-z_0)^2}+\frac{b_1}{z-z_0}+a_0+a_1(z-z_0)+\cdots  </mrow>
    </md>
    for all <m>z\in A</m>. Furthermore, letting <m>\gamma(t)=z_0+re^{it}</m> for any <m>r\in (R_1,R_2)</m> we have 
    <md>
        <mrow>a_n \amp =\frac{1}{2\pi i}\int_\gamma \frac{f(z)}{(z-z_0)^{n+1}}\, dz</mrow>
        <mrow>b_m \amp =\frac{1}{2\pi i}\int_\gamma f(z)(z-z_0)^{m-1}\, dz</mrow>
    </md>.
    Equivalently, for all <m>z\in A</m> we have 
    <me>
        f(z)=\sum_{n=-\infty}^\infty c_n(z-z_0)^n
    </me>,
    where 
    <men xml:id="eq_laurent_expansion">
        c_n=\frac{1}{2\pi i}\int_\gamma \frac{f(z)}{(z-z_0)^{n+1}}\, dz
    </men>.
    </p>
    </statement>
    <proof>
    <p>
        The proof is very simple to the proof of <xref ref="th_holo_implies_analytic"/>: the main fact we use is the Cauchy integral formula applied to elements within <m>A</m>. In more detail, given <m>w\in A</m>, pick a closed ball <m>\overline{B}_s(z_0)\subseteq A</m>, and let <m>\phi=w+se^{it}</m>, <m>t\in [0,2\pi]</m>. Next pick <m>R</m> and <m>S</m> satisfying <m>R_1&lt; R &lt; S &lt; R_2</m> such that <m>\overline{B}_s(z_0)</m> lies in the annular region <m>R&lt; \abs{z-z_0}&lt; S</m>, and let <m>\gamma_R(t)=z_0+Re^{it}</m> and <m>\gamma_S(t)=z_0+Se^{it}</m>, <m>t\in [0,2\pi]</m>. (See <xref ref="fig_laurent"/>.) By the Cauchy integral formula, we have 
        <me>
            f(w)=\frac{1}{2\pi i}\int_\phi \frac{f(z)}{z-w}\, dz
        </me>.
        By the principle of path deformation we have 
        <me>
          f(w)=\frac{1}{2\pi i}\int_\phi \frac{f(z)}{z-w}\, dz=\frac{1}{2\pi i}\int_{\gamma_S}\frac{f(z)}{z-w}\, dz-\frac{1}{2\pi i}\int_{\gamma_R}\frac{f(z)}{z-w}\, dz  
        </me>.
        Since <m>\abs{(w-z_0)/(z-w_0)}&lt; 1</m> for all <m>z\in \gamma_S</m>, we have 
        <md>
            <mrow>\frac{1}{2\pi i}\int_{\gamma_S}\frac{f(z)}{z-w}\, dw \amp = \frac{1}{2\pi i}\int_{\gamma_S}\frac{f(z)}{z-z_0}\cdot \frac{1}{1-(w-z_0)/(z-z_0)}\, dw </mrow>
            <mrow> \amp = \frac{1}{2\pi i}\int_{\gamma_S}(\frac{f(z)}{z-z_0}\sum_{n=0}^\infty((w-z_0)/(z-z_0))^n)\, dz</mrow>
            <mrow> \amp =\frac{1}{2\pi i} \sum_{n=0}^\infty\int_{\gamma_S}(\frac{f(z)}{(z-z_0)^{n+1}}\, dz)(w-z_0)^n</mrow>
            <mrow> \amp = \sum_{n=0}^\infty a_n(w-z_0)^n , \  a_n=\frac{1}{2\pi i}\int_{\gamma_S}\frac{f(z)}{(z-z_0)^n}\, dz</mrow>
        </md>.
        Similarly, since <m>\abs{(z-z_0)/(w-z_0)}&lt; 1</m> for all <m>z\in \gamma_R</m>, we have 
        <md>
            <mrow>\frac{1}{2\pi i}\int_{\gamma_R}\frac{f(z)}{z-w}\, dw \amp = \frac{1}{2\pi i}\int_{\gamma_R}\frac{f(z)}{w-z_0}\cdot \frac{-1}{1-(z-z_0)/(w-z_0)}\, dw </mrow>
            <mrow> \amp = -\frac{1}{2\pi i}\int_{\gamma_R}(\sum_{n=0}^\infty\frac{f(z)(z-z_0)^{n}}{(w-z_0)^{n+1}})\, dz</mrow>
            <mrow> \amp = -\frac{1}{2\pi i}\sum_{n=0}^\infty\int_{\gamma_R}(\frac{f(z)}{(z-z_0)^{n}}\, dz)(w-z_0)^{n+1}</mrow>
            <mrow> \amp = -\sum_{n=1}^\infty b_n(w-z_0)^{-n}, \  b_n=\frac{1}{2\pi i}\int_{\gamma_R}f(z)(z-z_0)^{n-1}\, dz</mrow>
        </md>.
        (Note that in both these computations we are justified in bringing the integral into the infinite sum thanks to the uniform convergence of this sum to the given function.)
    </p>
    <p>
        Putting it all together, we have 
        <md>
            <mrow> f(w)\amp =\frac{1}{2\pi i}\int_{\gamma_S}\frac{f(z)}{z-w}\, dz-\frac{1}{2\pi i}\int_{\gamma_R}\frac{f(z)}{z-w}\, dz</mrow>
            <mrow> \amp = \sum_{n=0}^\infty a_n(w-z_0)^n+\sum_{n=1}^\infty \frac{b_n}{(w-z_0)^n}</mrow>
        </md>
        for all <m>w\in A</m>, where (using the principle of deformation once again)
        <md>
            <mrow> a_n \amp=\frac{1}{2\pi i}\int_{\gamma_S}\frac{f(z)}{(z-z_0){n+1}}\, dz=\frac{1}{2\pi i}\int_{\gamma}\frac{f(z)}{(z-z_0){n+1}}\, dz </mrow>
            <mrow> b_n \amp=\frac{1}{2\pi i}\int_{\gamma_R}f(z)(z-z_0)^{n-1}\, dz=\frac{1}{2\pi i}\int_{\gamma}f(z)(z-z_0)^{n-1}\, dz </mrow>
        </md>.
        Recall that <m>\gamma(t)=z_0+re^{it}</m>, <m>t\in [0,2\pi]</m> for some <m>r\in (R_1,R_2)</m>. 
    </p>
    </proof>
    </theorem>
    <figure xml:id="fig_laurent">
        <caption>Visual idea behind proof of <xref ref="th_laurent"/></caption>
        <image width="50%">
            <shortdescription>Visual idea behind proof of theorem</shortdescription>
        <sageplot>
P=point((1,1),color="blue", size=60, ticks=[[],[]])
Q=point((2,2),color="blue", size=60)
C=circle((1,1),2.25,color="green")
D=circle((2,2), .5, color="green")
E=circle((1,1),.75, color="red")
F=circle((1,1),2.5, color="red")
G=circle((1,1),.85,color="green")
t1=text("$w$",(1.85,1.75),color="black", fontsize=14)
t2=text("$z_0$",(1.25,1.15),color="black", fontsize=14)
t3=text("$R_2$",(.75,2.5),color="black", fontsize=14)
t6=text("$R_1$",(.75,1.35),color="black", fontsize=14)
t4=text("$S$",(1.2+1.5/sqrt(2),1.2-1.5/sqrt(2)),color="black", fontsize=14)
t5=text("$s$",(1.85+.25/sqrt(2),2.15+.25/sqrt(2)),color="black", fontsize=14)
t7=text("$R$",(1.15-.4/sqrt(2),.85-.4/sqrt(2)),color="black", fontsize=14)
l1=line(((1,1),(1,3.5)),linestyle="dashed", color="black")
l2=line(((2,2),(2+.5/sqrt(2),2+.5/sqrt(2))),linestyle="dashed", color="black")
l3=line(((1,1),(1+2.25/sqrt(2),1-2.25/sqrt(2))),linestyle="dashed", color="black")
l4=line(((1,1),(1-.85/sqrt(2),1-.85/sqrt(2))),linestyle="dashed", color="black")
P+C+Q+D+t1+t2+l1+l2+E+l3+t3+t4+t5+F+t6+G+l4+t6+t7
        </sageplot>
        </image>
    </figure>
    
    <definition xml:id="d_laurent_series">
    <title>Laurent series</title>
    <statement>
    <p>
    Given <m>z_0\in \C</m>, a <term>(complex) laurent series centered at <m>z_0</m></term> in the variable <m>z</m> is an expression of the form 
    <men xml:id="eq_laurent_series">
    f(z)=\sum_{n=-\infty}^\infty c_n(z-z_0)^n= \cdots \frac{c_{-2}}{(z-z_0)^2}+\frac{c_{-1}}{z-z_0}+c_0+c_1(z-z_0)+c_2(z-z_0)^2+\cdots
    </men>,
    where <m>c_n\in \C</m>.  
    </p>
    <p>
        Let
        <mdn>
            <mrow xml:id="eq_laurent_g">g(u) \amp =\sum_{n=0}^\infty a_n u^n, a_n=c_n</mrow>
            <mrow xml:id="eq_laurent_h">h(u) \amp =\sum_{n=1}^\infty b_n u^n, b_n=c_{-n}</mrow>
        </mdn>
        so that 
        <me>
            f(z)=g(z-z_0)+h(1/(z-z_0))
        </me>.
        We say the Laurent series <m>f</m> <term>converges</term> at a complex number <m>z</m> if the series <m>g(z-z_0)</m> and <m>h(1/(z-z_0))</m> both converge, and <term>diverges</term> otherwise. In the case of convergence, we call <m>g(z-z_0)+h(1/(z-z_0))</m> the <term>value</term> of the Laurent series.  
    </p>
    </statement>
    </definition>
    <example xml:id="eg_laurent_essential">
    <title>Laurent series expansion</title>
    <statement>
    <p>
    Let <m>f(z)=z^3e^{1/z}</m>. Find a Laurent series expansion of <m>f</m> centered at <m>z_0=0</m> in the annulus
    <me>
        A=\{z\in \C\colon 0&lt; \abs{z} &lt; \infty\}=\C-\{0\}
    </me>.
    </p>
    </statement>
    <solution>
    <p>
    Since the power series representation 
    <me>
        e^{z}=\sum_{n=0}^\infty \frac{z^n}{n!}
    </me>
    is valid for all <m>z</m>, we have 
    <me>
        e^{1/z}=\sum_{n=0}^\infty \frac{1}{n! z^n}
    </me>
    and 
    <md>
        <mrow>z^3e^{1/z} \amp  =\sum_{n=0}^\infty \frac{1}{n!z^{n+3}}</mrow>  
        <mrow> \amp =z^3+z^2+\frac{1}{2}z+\frac{1}{6}+\frac{1}{24z}+\cdots  </mrow>
        <mrow> \amp = \sum_{n=-1}^\infty \frac{1}{(-n+3)!}z^{n}+ \frac{1}{2}+z^2+z^3</mrow>
    </md>
    for all <m>z\in \C-\{0\}</m>. 
    </p>
    </solution>
    </example>
    <remark>
    <title>Laurent series</title>
    <p>
    Since the notion of convergence of a Laurent series boils down to the convergence of the two power series <xref first="eq_laurent_g" last="eq_laurent_h"/>, Laurent series inherit many of the useful properties of power series. For example, from the uniform convergence properties of <m>g</m> and <m>h</m>, it follows that the Laurent series <m>f</m> can be differentiated and integrated term-wise, just as with power series. 
    </p>
    <p>
        As we saw in <xref ref="th_laurent"/>, however, the natural region of convergence of a Laurent series is an open annulus, as opposed to an open ball. Indeed, if the radii of convergence for <m>g</m> and <m>h</m> are <m>R</m> and <m>S</m>, respectively, then <m>g</m> converges at all <m>z</m> with <m>\abs{z-z_0}&lt; R</m> and <m>h</m> converges for all <m>z</m> with <m>\abs{1/(z-z_0)}&lt; S</m>. Letting <m>R'=1/S</m>, it follows that <m>f</m> converges for all <m>z</m> satisfying <m>R' &lt; \abs{z-z_0}&lt; R</m>, and diverges for all <m>z</m> satisfying <m>\abs{z-z_0}&lt; R'</m> or <m>\abs{z-z_0}&gt; R</m>. Accordingly, we call <m>A=\{z\in \C\colon R' &lt; \abs{z-z_0}&lt; R\}</m> the <term>annulus of convergence</term> of <m>f</m>.
    </p>
    </remark>
    <p>
        As a consequence of the discussion above, given a Laurent series, there is a well-defined annulus of convergence associated to it. As the next example illustrates, however, if we begin with a function <m>f</m> and seek out Laurent series expansions of <m>f</m>, these expansions depend on the annulus we choose. 
    </p>
    <example xml:id="eg_laurent_series">
    <title>Different Laurent series</title>
    <statement>
    <p>
    Let <m>f(z)=\frac{1}{z^2-4z+3}</m>. Compute a convergent Laurent series for <m>f</m> centered at <m>z_0=-1</m> in the given annulus <m>A</m>
    <ol>
        <li>
            <p>
                <m>A=\{z\in \C\colon 0&lt; \abs{z+1} &lt; 2\}</m>
            </p>
        </li>
        <li>
            <p>
                <m>A=\{z\in \C\colon 2&lt; \abs{z+1} &lt; 4\}</m>
            </p>
        </li>
        <li>
            <p>
                <m>A=\{z\in \C\colon 4&lt; \abs{z+1} &lt;\infty\}</m>
            </p>
        </li>
    </ol>
    </p>
    </statement>
    <solution>
    <p>
    We first use partial fractions to write 
    <me>
        f(z)=\frac{1}{(z-1)(z-3)}=-\frac{1}{2}\left(\frac{1}{z-1}-\frac{1}{z-3}\right)
    </me>. 
    Each computation below then boils down to deriving a Laurent series expansion of <m>1/(z-1)</m> and <m>1/(z-3)</m> in the given region. 
    <ol>
        <li>
            <p>
                If <m>0&lt; \abs{z+1} &lt; \abs{2}</m> then <m>\abs{(z+1)/2}&lt; 1</m> and <m>\abs{(z+1)/4}&lt; 1</m>. We maneuver into a place where we can use the geometric series for both fractions:
                <md>
                    <mrow>\frac{1}{z-1} \amp = \frac{1}{(z+1)-2}</mrow>
                    <mrow> \amp = -\frac{1}{2}\frac{1}{1-(z+1)/2}</mrow>
                    <mrow> \amp = -\frac{1}{2}\sum_{n=0}^\infty \frac{1}{2^n}(z+1)^n</mrow>
                    <mrow>\frac{1}{z-3} \amp = \frac{1}{(z+1)-4}</mrow>
                    <mrow> \amp = -\frac{1}{4}\frac{1}{1-(z+1)/4}</mrow>
                    <mrow> \amp = -\frac{1}{4}\sum_{n=0}^\infty \frac{1}{4^n}(z+1)^n</mrow>
                </md>
                We conclude that 
                <md>
                    <mrow>f(z) \amp = -\frac{1}{2}\left(\frac{1}{z-1}-\frac{1}{z-3}\right) </mrow>
                    <mrow> \amp = \frac{1}{4}\sum_{n=0}^\infty \frac{1}{2^n}(z+1)^n-\frac{1}{8}\sum_{n=0}\frac{1}{4^n}(z+1)^n</mrow>
                    <mrow> \amp = \frac{1}{2}\sum_{n=0}^\infty \frac{2^{n+1}-1}{4^{n+1}}(z+1)^n  </mrow>
                </md>.
                It should come as no surprise that our Laurent series expansion in this case is a power series, as <m>f</m> is in fact analytic on the entire ball <m>\abs{z+1}&lt; 2</m>. 
            </p>
        </li>
        <li>
            <p>
               For <m>z</m> satisfying <m>2&lt; \abs{z+1} &lt; 4</m>, we may continue to use our power series expansion for the second fraction, but not the first, since now <m>\abs{(z+1)/2}&gt; 1</m>. But of course, this is equivalent to <m>\abs{2/(z+1)}&lt; 1</m>. So we maneuver accordingly:
               <md>
                    <mrow>\frac{1}{z-1} \amp = \frac{1}{(z+1)-2}</mrow>
                    <mrow> \amp = \frac{1}{z+1}\frac{1}{1-2/(z+1)}</mrow>
                    <mrow> \amp = \sum_{n=0}^\infty \frac{2^n}{(z+1)^{n+1}}</mrow>
                    <mrow>\frac{1}{z-3} \amp = -\frac{1}{4}\sum_{n=0}^\infty \frac{1}{4^n}(z+1)^n</mrow>
                </md>
               Thus 
               <md>
                <mrow> f(z)\amp =-\frac{1}{2}\left(\frac{1}{z-1}-\frac{1}{z-3}\right) </mrow>
                <mrow> \amp = -\frac{1}{2}\sum_{n=0}^\infty \frac{2^n}{(z+1)^{n+1}} -\frac{1}{8}\sum_{n=0}^\infty \frac{1}{4^n}(z+1)^n  </mrow>
               <mrow> \amp = -\sum_{n=0}^\infty \frac{2^{n-1}}{(z+1)^{n+1}} -\frac{1}{8}\sum_{n=0}^\infty \frac{1}{4^n}(z+1)^n  </mrow>
               <mrow> \amp = -\sum_{n=1}^\infty \frac{2^{n-2}}{(z+1)^{n}} -\frac{1}{8}\sum_{n=0}^\infty \frac{1}{4^n}(z+1)^n  </mrow>
               </md>.
            </p>
        </li>
        <li>
            <p>
                Finally, for <m>\abs{z+1}&gt; 4</m>, we have <m>\abs{2/(z+1)}&lt; 1</m> and <m>\abs{4/(z+1)}&lt; 1</m>, yielding (similarly as above)
                <md>
                    <mrow>\frac{1}{z-1} \amp = \sum_{n=0}^\infty \frac{2^n}{(z+1)^{n+1}}</mrow>
                    <mrow>\frac{1}{z-3} \amp = \sum_{n=0}^\infty\frac{4^n}{(z+1)^{n+1}}</mrow>
                </md>
                and thus 
                <md>
                    <mrow>f(z) \amp = \frac{1}{2}\sum_{n=0}^\infty\frac{4^n}{(z+1)^{n+1}} - \frac{1}{2}\sum_{n=0}^\infty \frac{2^n}{(z+1)^{n+1}}</mrow>
                    <mrow> \amp = \frac{1}{2}\sum_{n=0}^\infty \frac{4^n-2^n}{(z+1)^{n+1}}</mrow>
                    <mrow> \amp = \sum_{n=1}^\infty \frac{2^{n-2}(2^{n-1}-1)}{(z+1)^n}</mrow>
                </md>.
            </p>
        </li>
    </ol>
    </p>
    </solution>
    </example>
    <remark>
        <title>Multiplying power series</title>
       <p>
        The next example requires multiplying together two power series. In general, given two power series 
        <md>
            <mrow>f(z) \amp = \sum_{n=0}^\infty a_n(z-z_0)^n \amp g(z)\amp =\sum_{n=0}^\infty b_n(z-z_0)^n</mrow>
        </md>
        that converge for all <m>z\in B_R(z_0)</m>, their product has power series expansion
        <me>
            f(z)g(z)=\sum_{n=0}^\infty c_n(z-z_0)^n
        </me>,
        where 
        <me>
            c_n=a_0b_n+a_1b_{n-1}+\cdots a_nb_0=\sum_{k=0}^na_kb_{n-k}
        </me>.
       </p> 
        
    </remark>
    <example xml:id="eg_laurent_series_trunc">
    <title>Truncated Laurent series</title>
    <statement>
    <p>
    Let <m>A</m> be the annulus <m>0&lt; \abs{z} &lt; 1</m>. Compute the Laurent series <m>\sum_{n=-\infty}^\infty c_n z^n</m> of <m>f(z)=e^z/(z^3+z^2)</m> in <m>A</m> up through <m>c_2</m>. 
    </p>
    </statement>
    <solution>
    <p>
    We have 
    <md>
        <mrow>f(z) \amp =\frac{e^z}{z^2(z+1)}</mrow>
        <mrow> \amp = \frac{1}{z^2}\cdot (1+z+\frac{z^2}{2}+\frac{z^3}{6}+\cdots)(1-z+z^2-z^3+\cdots)</mrow>
        <mrow> \amp = \frac{1}{z^2}\sum_{n=0}^\infty c_n z^n, \ c_n=\sum_{k=0}^n(-1)^{n-k}/n!</mrow>
        <mrow> \amp = \frac{1}{z^2}(1+0z+\frac{1}{2}z^2-\frac{1}{3}z^3+\frac{3}{8}z^4+\cdots)</mrow>
        <mrow> \amp = \frac{1}{z^2}+\frac{1}{2}-\frac{1}{3}z+\frac{3}{8}z^2+\cdots</mrow>
    </md>
    </p>
    </solution>
    </example>
    <remark>
        <title>Expanding a polynomial about a different center</title>
        <p>
            Since a polynomial <m>f(z)=a_nz^n+a_{n-1}z^{n-1}+\cdots +a_1z+a_0</m> is entire, we can expand it as a power series about any center <m>z_0</m>. We see using formula <xref ref="eq_power_series_coeff_formula"/> that 
            <md>
                <mrow>f(z) \amp = \sum_{k=0}^\infty c_k(z-z_0)^k </mrow>
                <mrow> \amp = \sum_{k=0}^\infty \frac{f^{(k)}(z_0)}{k!}(z-z_0)^k</mrow>
                <mrow> \amp = f(z_0)+f'(z_0)(z-z_0)+\frac{f''(z_0)}{2}(z-z_0)^2+\cdots +\frac{f^{(n)}(z_0)}{n!}(z-z_0)^n</mrow>
            </md>,
            since <m>f^{(k)}</m> is the zero function for all <m>k\geq n+1</m>. 
        </p>
        
    </remark>
    <example xml:id="eg_laurent_series_rational">
    <title>Laurent series of rational function</title>
    <statement>
    <p>
    Let <m>A</m> be the annulus <m>0&lt; \abs{z-1} &lt; \infty</m>: <ie/>, <m>A=\C-\{1\}</m>. Compute the Laurent series of <m>f(z)=(z^3+2z^2)/(z-1)^3</m> on <m>A</m>. 
    </p>
    </statement>
    <solution>
    <p>
    Let <m>g(z)=z^3+2z^2</m>. We first expand <m>g</m> about <m>z_0=1</m> as 
    <md>
        <mrow> g(z)\amp =g(1)+g'(1)(z-1)+\frac{g''(0)}{2!}(z-1)^2+\frac{g'''(0)}{3!}(z-1)^3</mrow>
        <mrow> \amp =3+7(z-1)+5(z-1)^2+(z-1)^3\amp </mrow>
    </md>.
    Now compute 
    <md>
        <mrow>f(z) \amp = \frac{g(z)}{(z-1)^3}=\frac{3}{(z-1)^3}+\frac{7}{(z-1)^2}+\frac{5}{z-1}+1</mrow>
    </md>.
    </p>
    </solution>
    </example>
    
    
    

</section>