<?xml version="1.0" encoding="UTF-8"?>

<section xml:id="s_log_trig" xmlns:xi="http://www.w3.org/2001/XInclude">
    <title>Logarithmic and trigonometric functions</title>

    <introduction>
        <p>
            
        </p>
    </introduction>
<subsection xml:id="ss_log">
<title>Logarithmic functions</title>
<p>
    When showing that <m>\exp\colon \C\rightarrow \C</m> has image <m>\C-\{0\}</m>, we showed that for any <m>z\in \C-\{0\}</m>, the set of solutions to <m>e^w=z</m> is the set 
    <me>
        \{w\in \C\colon \Re w=\ln \abs{z} \text{ and } \Im w\in \arg(z)\}=\{\ln\abs{z}+i(\Arg z+2\pi k)\colon k\in \Z\}
    </me>.
    This motivates the following definition. 
</p>
    <definition xml:id="d_log">
    <title>Logarithm</title>
    <statement>
    <p>
    Given <m>z\in \C-\{0\}</m>, we define the <term>logarithm</term> of <m>z</m>, denoted <m>\log z</m>, to be the infinite set 
    <me>
        \log z=\{w\in \C\colon \Re w=\ln \abs{z} \text{ and } \Im w\in \arg(z)\}=\{\ln\abs{z}+i(\Arg z+2\pi k)\colon k\in \Z\}
    </me>.
    The <term>principal branch of the logarithm</term> is the function <m>\Log\colon \C-(-\infty,0]\rightarrow \C</m> defined as 
    <me>
        \Log z=\ln\abs{z}+i\Arg z
    </me>
    </p>
    </statement>
    </definition>
    <remark>
        <p>
            Using the same sort of shorthand as in <xref ref="rm_solve_exp"/>, we can write 
            <md>
                <mrow>\log z \amp = \ln\abs{z}+i\arg z</mrow>
            </md>,
            where as always 
            <me>
                \arg z=\{\Arg z+2\pi k\colon k\in \Z\}
            </me>
            is the set of all arguments of <m>z</m>.
        </p>
    </remark>
    <remark>
        <title><m>\Log</m></title>
        <p>
            We will see in due course that there is a good reason for the funny domain specified for <m>\Log z</m>. Namely, although we can in principle define <m>\Log z</m> for any <m>z\ne 0</m>, the domain <m>\C-(-\infty, 0]</m> ensures that <m>\Log z</m> is continuous, and is in a sense maximal in this regard. 
        </p>
    </remark>
    <theorem xml:id="th_exp_Log">
    <title><m>\Log</m> as inverse function</title>
    <statement>
    <p>
    Let <m>R=\{z\in \C\colon -\pi&lt; \Im z &lt; \pi\}</m>, and define <m>f\colon R\rightarrow \C-(-\infty,0]</m> as <m>f(z)=e^z</m>: <ie/>, <m>f</m> is the restriction of <m>\exp</m> to the set <m>R</m>. The function <m>\Log\colon \C-(-\infty, 0]\rightarrow R</m> is the inverse of <m>f</m>: <ie/>, we have 
    <mdn>
        <mrow xml:id="eq_log_exp">\Log(e^z) \amp = z \text{ for all } z\in R</mrow>
        <mrow xml:id="eq_exp_log">e^{\Log(w)} \amp = w \text{ for all } w\in \C-(-\infty, 0]</mrow>
    </mdn>.
    </p>
    </statement>
    <proof>
    <p>
        Recall that we remarked in the discussion above <xref ref="fig_exp_trans_strip"/> that the given <m>f</m> is a bijection, and hence invertible; the theorem claims that <m>\Log</m> is the inverse of this function. First observe that <m>\im \Log\subseteq R</m>, since
        <md>
            <mrow>w\in \C-(-\infty,0] \amp \implies -\pi&lt; \Arg w &lt; \pi</mrow>
            <mrow> \amp\implies -\pi &lt; \Im(\Log z) &lt; \pi</mrow>
            <mrow> \amp \implies \Log z\in R</mrow>
        </md>.
        The identities <xref first="eq_log_exp" last="eq_exp_log"/> are easily verified using the formulas for <m>\exp</m> and <m>\Log</m> applied to elements in <m>R</m> and <m>\C-\{0\}</m>. 
    </p>
    </proof>
    </theorem>
    
    <example xml:id="eg_log">
    <title>Logarithm</title>
    <statement>
    <p>
    Compute <m>\log z</m> and <m>\Log z</m> (if applicable) for the given <m>z</m>. 
    <ol>
        <li>
            <p>
                <m>z=3</m>
            </p>
        </li>
        <li>
            <p>
                <m>z=-2</m>
            </p>
        </li>
        <li>
            <p>
                <m>z=1+i</m>. 
            </p>
        </li>
    </ol>
    </p>
    </statement>
    <solution>
    <p>
    <ol>
        <li>
            <p>We have 
                <md>
                    <mrow>\log 3 \amp =\ln 3+i\arg(3)=\{\ln 3+2\pi k i\colon k\in \Z\}</mrow>
                    <mrow>\Log 3 \amp =\ln 3</mrow>
                </md>.
            </p>
        </li>
        <li>
            <p>We have 
               <md>
                <mrow>\log(-2) \amp = \ln\abs{-2}+i\arg(-2)</mrow>
                <mrow> \amp = =\ln 2+i\arg(-2)</mrow>
                <mrow> \amp = \{\ln 2+i(\pi +2\pi k)\colon k\in \Z\}</mrow>
                <mrow> \amp = \{\ln 2+(2k+1)\pi i \colon k\in \Z\}</mrow>
               </md>.
               Technically, <m>\Log</m> is not defined at <m>z=-2</m>. 
            </p>
        </li>
        <li>
            <p>We have 
                <md>
                    <mrow>\log(1+i) \amp = \ln(\sqrt{2})+i\arg(1+i)</mrow>
                    <mrow> \amp = \{\ln(\sqrt{2})+i(\pi/4+2\pi k)\colon k\in \Z\}</mrow>
                    <mrow>\Log(1+i) \amp = \ln(\sqrt{2})+\frac{\pi i}{4}</mrow>
                </md>.
            </p>
        </li>
    </ol>
    </p>
    </solution>
    </example>
    <example xml:id="eg_Log">
    <title>Invalid identity</title>
    <statement>
    <p>
    Show that <m>\Log(z_1z_2)</m> is not always equal to <m>\Log(z_1)+\Log(z_2)</m>. 
    </p>
    </statement>
    <solution>
    <p>
    In general we have 
    <md>
        <mrow>\Log(z_1z_2) \amp = \ln\abs{z_1z_2}+i\Arg(z_1z_2)</mrow>
        <mrow> \amp =(\ln\abs{z_1}+\ln\abs{z_2})+i\Arg(z_1z_2)</mrow>
        <mrow>\Log z_1+\Log z_2 \amp = (\ln\abs{z_1}+\ln\abs{z_2})+i(\Arg z_1+\Arg z_2)</mrow>
    </md>.
    The issue preventing equality to hold in general is that 
    <me>
        \Arg(z_1z_2)\ne \Arg(z_1)+\Arg(z_2)
    </me>.
    Indeed, taking <m>z_1=e^{\pi i/2}</m> and <m>z_2=e^{3\pi i/4}</m>, we have 
    <md>
        <mrow>\Arg(z_1z_2) \amp = \Arg(e^{5\pi i /4})=-\frac{3\pi}{4}</mrow>
        <mrow>\Arg(z_1)+\Arg(z_2) \amp =\frac{\pi}{2}+\frac{3\pi }{4}=\frac{5\pi}{4}</mrow>
    </md>.
    </p>
    </solution>
    </example>
</subsection>
<subsection xml:id="ss_power">
<title>Complex exponentiation</title>
<definition xml:id="d_complex_exponentiation">
    <title>Complex exponentiation</title>
    <statement>
        <p>
            Given <m>z\in \C-\{0\}</m> and any <m>w\in \C</m>, we define the set <m>z^w</m> as 
            <me>
                z^w=e^{w\log z}
            </me>.
            Given a fixed <m>w\in \C</m>, the function <m>f\colon \C-(-\infty, 0]\rightarrow \C</m> defined as <m>f(z)=e^{w\Log z}</m> is called the <term>principal branch of the power function with exponent <m>w</m></term> (or <term>principal branch of <m>f(z)=z^w</m></term>). 
        </p>
    </statement>
</definition>
<example xml:id="eg_powers">
<title>Powers</title>
<statement>
<p>
Compute the following power expressions. 
<ol>
    <li>
        <p>
            <m>i^i</m>
        </p>
    </li>
    <li>
        <p>
            <m>z^i</m>, <m>z\ne 0</m>. 
        </p>
    </li>
</ol>
</p>
</statement>
<solution>
<p>

</p>
</solution>
</example>
<example xml:id="eg_nth_roots">
<title><m>n</m>-th roots</title>
<statement>
<p>
Let <m>z\ne 0</m>. Show that the set <m>z^{1/n}</m> is precisely the set of <m>n</m> distinct <m>n</m>-th roots of <m>z</m>. 
</p>
</statement>
<solution>
<p>

</p>
</solution>
</example>


</subsection>
<subsection xml:id="ss_trig">
    <p>
    Given a real number <m>t\in \R</m>, from the identity 
    <me>
        e^{it}=\cos t+i\sin t
    </me>
    and our formulas 
    <md>
        <mrow>\Re z \amp =\frac{z+\overline{z}}{2} \amp \Im z\amp \frac{z-\overline{z}}{2i}</mrow>
    </md>
    it follows that 
    <md>
        <mrow>\cos t\amp =\frac{e^{it}+e^{-it}}{2} \amp \sin t\amp =\frac{e^{it}-e^{-it}}{2i} </mrow>
    </md>.
    It is then natural to extend these formulas for all complex numbers <m>z</m>, yielding our definitions for the complex cosine and sine functions: 
    <md>
        <mrow> \cos z\amp =\frac{e^{iz}+e^{-iz}}{2} \amp \sin z\amp =\frac{e^{iz}-e^{-iz}}{2i} </mrow>
    </md>
    
    </p>
<title>Trigonometric functions</title>
<definition xml:id="d_trig_functions">
<title>Trigonometric functions</title>
<statement>
<p>
We define the <term>complex cosine and sine</term> <m>\cos\colon \C\rightarrow \C</m> and <m>\sin\colon \C\rightarrow \C</m> as follows: 
<mdn>
    <mrow xml:id="eq_cos">\cos(z) \amp = \frac{e^{iz}+e^{-iz}}{2} \amp </mrow>
    <mrow xml:id="eq_sin">\sin(z)\amp =\frac{e^{iz}-e^{-iz}}{2i}  </mrow>
</mdn>.
We then further define complex extensions of the other elementary trigonometric functions in the usual way:
<md>
    <mrow>\tan z \amp = \frac{\sin z}{\cos z} \amp \cot z\amp = \frac{\cos z}{\sin z}</mrow>
    <mrow>\sec z \amp = \frac{1}{\cos z} \amp \csc z\amp =\frac{1}{\sin z}</mrow>
</md>.
</p>
</statement>
</definition>
<theorem xml:id="th_trig_props">
<title>Cosine and sine properties</title>
<statement>
<p>
Let <m>z,w\in \C</m>. 
<ol>
    <li>
        <p>
            <m>\cos z=\cos w</m> if and only if <m>z=w+2\pi k</m> for some <m>k\in \Z</m>, or <m>z=-w+2\pi k</m> for some <m>k\in \Z</m>. 
        </p>
    </li>
    <li>
        <p>
            <m>\sin z=\sin w</m> if and only if <m>z=w+2\pi k</m> for some <m>k\in \Z</m> or <m>z=\pi-w+2\pi k</m> for some <m>k\in \Z</m>. 
        </p>
    </li>
    <li>
        <p>For all <m>z,w\in \C</m> we have 
            <mdn>
            <mrow>\cos^2 z+\sin^2 z \amp = 1 \amp \tan^2 z+1 \amp =\sec^2 z </mrow>
                <mrow xml:id="eq_angle_sum">\cos(z+w) \amp = \cos(z)\cos(w)-\sin(z)\sin(w) \amp 
                \sin(z+w) \amp =\sin z\cos w+\cos z\sin w </mrow>
                <mrow>\cos(2z) \amp = \cos^2 z-\sin^2 z \amp \sin(2z)\amp = 2\sin z\cos z</mrow>
            </mdn>.
        </p>
    </li>
</ol>
</p>
</statement>
<proof>
<p>
    <ol>
        <li>
            <p>
                Given <m>z,w\in \C</m>, we have 
                <md>
                    <mrow>\cos z=\cos w \amp \iff e^{iz}+e^{-iz}=e^{iw}+e^{-iw}</mrow>
                    <mrow> \amp \iff e^{iw}e^{iz}+e^{iw}e^{-iz}=e^{iw}e^{iw}+e^{iw}e^{-iw}</mrow>
                    <mrow> \amp \iff e^{i(z+w)}+e^{-i(z-w)}=e^{iw+iz}e^{iw-iz}+1</mrow>
                    <mrow> \amp \iff e^{i(z+w)}+e^{-i(z-w)}=e^{i(z+w)}e^{-i(z-w)}+1</mrow>
                    <mrow> \amp \iff e^{i(z+w)}(1-e^{-i(z-w)})-(1-e^{-i(z-w)})=0</mrow>
                    <mrow> \amp \iff (1-e^{-i(z-w)})(e^{i(z+w)}-1)=0 </mrow>
                    <mrow> \amp \iff e^{-i(z-w)}=1 \text{ or } e^{i(z+w)}=1</mrow>
                </md>.
                Next since <m>e^u=1</m> if and only if <m>u=0+2\pi k i</m> for some <m>k\in \Z</m>, we see that <m>\cos z=\cos w</m> if and only if 
                <md>
                    <mrow>-i(z-w)\amp =2\pi k i \text{ for some } k\in \Z </mrow>
                    <mrow>\amp \text{ or } </mrow>
                    <mrow>i(z+w)\amp =2\pi k i \text{ for some } k\in \Z </mrow>
                </md>
                if and only if 
                <md>
                    <mrow>z\amp =w+2\pi k  \text{ for some } k\in \Z </mrow>
                    <mrow>\amp \text{ or } </mrow>
                    <mrow>z\amp=-w +2\pi k  \text{ for some } k\in \Z </mrow>
                </md>,
                as claimed. 
            </p>
        </li>
        <li>
            <p>
                The proof of this statement is very similar to the one above. 
            </p>
        </li>
        <li>
            <p>
                These identities can be proved in a straightforward manner using the the defining formulas <xref first="eq_cos" last="eq_sin"/> and properties of complex multiplication. 
            </p>
        </li>
    </ol>
</p>
</proof>
</theorem>
<definition xml:id="d_hyperbolic">
<title>Complex hyperbolic functions</title>
<statement>
<p>
We define the <term>complex hyperbolic functions</term> <m>\cosh\colon \C\rightarrow \C</m> and <m>\sinh\colon \C\rightarrow \C</m> as follows: 
<md>
    <mrow>\cosh(z) \amp =\frac{e^z+e^{-z}}{2} \amp \sinh(z)=\frac{e^{z}-e^{-z}}{2}</mrow>
</md>.
</p>
</statement>
</definition>
<theorem xml:id="th_hyperbolic">
<title>Complex hyperbolic functions</title>
<statement>
<p> 
<ol>
    <li>
        <p> For all <m>z\in \C</m> we have 
        <md>
            <mrow>\cosh(z) \amp = \cos(iz) \amp \sinh(z)\amp= \frac{\sin(iz)}{i}</mrow>
        </md>.
        </p>
    </li>
    <li>
        <p>
            For all <m>z=x+iy\in \C</m> we have 
            <md>
                <mrow>\cos(z) \amp =\cos(x)\cosh(y)-i\sin(x)\sinh(y)</mrow>
                <mrow>\sin(z) \amp =\sin(x)\cosh(y)+i\cos(x)\sinh(y)</mrow>
            </md>.
        </p>
    </li>
</ol>
</p>
</statement>
<proof>
<p>
    <ol>
        <li>
            <p>
                These identities follow directly from <xref ref="d_trig_functions"/> and <xref ref="d_hyperbolic"/>. 
            </p>
        </li>
        <li>
            <p>
                These identities follow directly from the sum identities in <xref ref="eq_angle_sum"/> and <xref ref="d_hyperbolic"/>. 
            </p>
        </li>
    </ol>
</p>
</proof>
</theorem>

</subsection>
</section>