<?xml version="1.0" encoding="UTF-8"?>

<section xml:id="s_power_series" xmlns:xi="http://www.w3.org/2001/XInclude">
    <title>Complex power series</title>

    <definition xml:id="d_power_series">
    <title>Complex power series</title>
    <statement>
    <p>
    Given <m>z_0\in \C</m>, a <term>(complex) power series centered at <m>z_0</m></term> in the variable (or unknown) <m>z</m> is an expression of the form 
    <men xml:id="eq_power_series">
    f(z)=\sum_{n=0}^\infty a_n(z-z_0)^n=a_0+a_1(z-z_1)+a_2(z-z_0)^2+\cdots
    </men>, where <m>a_n\in \C</m>. We call <m>z_0</m> the <term>center</term> of the power series, and <m>a_n</m> the <m>n</m>-th <term>coefficient</term> of the series. 
    </p>
    <p>
        For any integer <m>k\geq 0</m>, the <term><m>k</m>-th partial sum</term> of the power series <m>f</m> is the function <m>f_k(z)</m> defined as 
        <me>
            f_k(z)=\sum_{n=0}^ka_nz^n
        </me>.
    </p>
    <p>
        Given <m>w\in \C</m>, we say the power series <m>f(z)=\sum_{n=0}^{\infty}a_n(z-z_0)^n</m> <term>converges</term> (resp. <term>diverges</term>) at <m>w</m> if the infinite series <m>f(w)=\sum_{n=0}^{\infty}a_n(w-z_0)^n</m> converges (resp. diverges).
    </p>
    </statement>
    </definition>
    <p>
        Recall the geometric series <m>f(z)=\sum_{n=0}^\infty z^n</m> treated in <xref ref="eg_geom_series"/>. We saw there that the series converges for all <m>z</m> with <m>\abs{z}&lt; 1</m> and showed that for all such <m>z</m> we have 
        <men xml:id="eq_geom_series">
            f(z)=\sum_{n=0}^\infty z^n=\frac{1}{1-z}
        </men>.
        We also showed that the series diverges for all <m>z</m> with <m>\abs{z}&gt; 0</m> (as well as for all <m>z</m> with <m>\abs{z}=1</m>). Make this example your friend. It is both one of the simplest power series and one of the most fundamental, and will show up with an uncanny persistence.
    </p>
    <p>
        The formula for the function <m>f(z)=\frac{1}{1-z}</m> given in <xref ref="eq_geom_series"/> is an example of a <em>power series representation</em> of <m>f</m> on the open set <m>B_1(0)</m>. 
    </p>
    <definition xml:id="d_power_series_expansion">
    <title>Power series representation</title>
    <statement>
    <p>
    Given a complex function <m>f</m> defined on the open set <m>U</m>, a <term>power series representation</term> (or <term>expansion</term>) of <m>f</m> on <m>U</m> is a power series <m>\sum_{n=0}^\infty a_n(z-z_0)^n</m> that satisfies 
    <me>
        f(z)=\sum_{n=0}^{\infty}a_n(z-z_0)^n
    </me>
    for all <m>z\in U</m>. 
    </p>
    </statement>
    </definition>
    <p>
        We will be able to generate many power series representations of functions from the geometric series, as the next example indicates. 
    </p>
    <example xml:id="eg_power_series">
    <title>Power series representation</title>
    <statement>
    <p>
    Find a power series representation of the given function, centered at the given <m>z_0</m>. 
    Let <m>f(z)=\frac{z^3}{9-z^2}</m>. Find power series representation of <m>f</m> centered at <m>z_0=0</m> on the open set <m>U=B_3(0)</m>.  
    </p>
    </statement>
    <solution>
    
            <p>
                We have 
                <md>
                    <mrow>f(z) \amp =\frac{z^3}{9}\cdot \frac{1}{1-(z/3)^2}</mrow>
                </md>.
                Since formula <xref ref="eq_geom_series"/> is valid for <em>all</em> complex in <m>B_1(0)</m>, we have 
                <me>
                    \frac{1}{1-(z/3)^2}=\sum_{n=0}^\infty((z/3)^2)^n=\sum_{n=0}^\infty \frac{1}{3^{2n}}z^{2n}
                </me>
                for all <m>z</m> with <m>\abs{(z/3)^2}&lt; 1</m>, and thus for all <m>z</m> with <m>\abs{z}&lt; 3</m>. Using the product law for limits, it follows that 
                <me>
                    f(z)=\frac{z}{9}\sum_{n=0}^\infty \frac{1}{3^{2n}}z^{2n}=\sum_{n=0}^\infty\frac{1}{3^{2n+2}}z^{2n+1}
                </me>.
            </p>
    </solution>
    </example>
    <p>
        <xref ref="th_powerseries_conv"/> details not only where a power series converges, but also <em>how</em> it converges. The latter discussion touches on the notion of uniform convergence of sequences of functions, which we now officially introduce. 
    </p>
    <definition xml:id="d_function_convergence">
    <title>Sequences of functions</title>
    <statement>
    <p>
    Let <m>(f_n)_{n=0}^\infty</m> be a sequence of complex functions of the form <m>f_n\colon D\rightarrow \C</m>.
    <ul>
        <li>
            <title>Pointwise convergence</title>
            <p>
                The sequence <m>(f_n)</m> is said to <term>converge pointwise</term> to a function <m>f\colon D\rightarrow \C</m> if for all <m>z\in D</m> we have <m>f_n(z)\to f(z)</m>: <ie/>, for all <m>z\in D</m> and <m>\epsilon &gt; 0</m>, there exists an integer <m>N\geq 0</m> such that <m>\abs{f_n(z)-f(z)}&lt; \epsilon</m> for all <m>n\geq N</m>. We write <m>\lim\limits_{n\to \infty}f_n=f</m> or <m>f_n\to f</m> when this is the case. 
            </p>
        </li>
        <li>
            <title>Uniform convergence</title>
            <p>
                The sequence <m>(f_n)</m> is said to <term>converge uniformly</term> to a function <m>f\colon D\rightarrow \C</m> if for all <m>\epsilon &gt; 0</m>, there exists an integer <m>N\geq 0</m> such that for all <m>z\in D</m> and for all <m>n\geq N</m>, <m>\abs{f_n(z)-f(z)}&lt; \epsilon</m>.
            </p>
        </li>
    </ul>  
    </p>
    </statement>
    </definition>
    <theorem xml:id="th_powerseries_conv">
    <title>Power series convergence</title>
    <statement>
    <p>
    Let <m>f(z)=\sum_{n=0}^\infty a_n (z-z_0)^n</m> be a complex power series and suppose <m>f</m> converges at <m>w_0\in \C</m>. Let <m>R=\abs{w_0-z_0}</m>. 
    <ol>
        <li>
            <title>Absolute convergence</title>
            <p>
                For all <m>z\in B_{R}(z_0)</m> the infinite series <m>f(z)</m> converges absolutely.
            </p>
        </li>
        <li>
            <title>Uniform convergence</title>
            <p>
                For all integers <m>k\geq 0</m>, let <m>f_k(z)=\sum_{n=0}^ka_nz^n</m> be the <m>k</m>-th partial sum of <m>f</m>. Given any <m>r</m> with <m>0&lt; r&lt; R</m> the sequence of partial sums <m>(f_k)_{k=0}^{\infty}</m> converges to <m>f</m> uniformly on <m>\overline{B}_r(z_0)</m>.
            </p>
        </li>
    </ol>
    </p>
    </statement>
    <proof>
    <p>
        We first observe that since <m>f(w_0)=\sum_{n=0}^\infty a_n(w_0-z_0)^n</m> converges, we have 
        <me>
            \abs{a_n (w_0-z_0)^n}\to 0
        </me>,
        and this in turn implies that there is an <m>M\geq 0</m> such that <m>\abs{a_n (w_0-z_0)^n}\leq M</m> for all <m>n</m>.         
        <ol>
            <li>
                <p>
                    Let <m>w\in B_R(z_0)</m>. We will show that 
                    <me>
                        \sum_{n=0}^\infty \abs{a_n(w-z_0)^n}
                    </me>
                    converges by comparing it to a certain geometric series. Namely, we have 
                    <md>
                        <mrow>\abs{a_n(w-z_0)^n} \amp =\abs{a_n(w_0-z_0)^n\left(\frac{w-z_0}{w_0-z_0}\right)^n}</mrow>
                        <mrow> \amp = \abs{a_n(w_0-z_0)^n}\abs{\frac{w-z_0}{R}}^n </mrow>
                        <mrow> \amp \leq M\abs{\frac{w-z_0}{R}}^n</mrow>
                    </md>,
                    where <m>M</m> is the bound on <m>\abs{a_n(w_0-z_0)^n</m> discussed above. 
                    Since <m>w\in B_R(z_0)</m>, we have <m>\abs{(w-z_0)/r}&lt; 1</m>, and thus the geometric series 
                    <me>
                        \sum_{n=0}^\infty M \abs{\frac{w-z_0}{R}}^n
                    </me>
                    converges. It follows by the comparison test that <m>\sum_{n=0}^\infty \abs{a_n(w-w_0)^n}</m> converges. Thus <m>f(w)</m> is absolutely convergent.
                </p>
            </li>
            <li>
                <p>
                    First observe that for all <m>z\in B_R(z_0)</m> we have
                    <md>
                        <mrow>\abs{f_k(z)-f(z)} \amp = \abs{f(z)-f_k(z)}</mrow>
                        <mrow> \amp = \abs{\sum_{n=0}^\infty a_n(z-w_0)^n-\sum_{n=k}^\infty a_n(z-w_0)^n}</mrow>
                        <mrow> \amp = \abs{\sum_{n=k+1}^\infty a_n(z-w_0)^n}</mrow>
                    </md>
                    for all integers <m>k\geq 0</m>. Fix any <m>r</m> with <m>0 &lt; r &lt; R</m>. Given any <m>z\in B_r(z_0)</m>,  arguing exactly as above, we have 
                    <md>
                    <mrow> \abs{\sum_{n=k+1}^\infty a_n(z-w_0)^n}\amp \leq \sum_{n=k+1}^\infty \abs{a_n(z-w_0)^n}</mrow>
                    <mrow> \amp \leq \sum_{n=k+1}^\infty M\abs{\frac{z-z_0}{w_0-z_0}}^n</mrow>
                    <mrow> \amp = M\sum_{n=k+1}^\infty (r/R)^n</mrow>
                    <mrow> \amp = M(r/R)^k\sum_{n=0}^\infty (r/R)^n</mrow>
                    <mrow> \amp = M(r/R)^k\cdot \frac{1}{1-(r/R)}</mrow>
                    <mrow> \amp =(r/R)^k\cdot \frac{MR}{R-r}</mrow>
                    </md>,
                    since <m>r/R&lt; 1</m>. Since <m>M</m>, <m>R</m>, and <m>r</m> are fixed constants, we see that 
                    <me>
                        (r/R)^k\cdot \frac{MR}{R-r}\to 0
                    </me>
                    as <m>k\to \infty</m>. It follows that for any <m>\epsilon &gt; 0</m> we can find an integer <m>N\geq 0</m> such that <m>k\geq N</m> implies 
                    <me>
                        (r/R)^k\cdot \frac{MR}{R-r}&lt; \epsilon
                    </me>.
                    We conclude that for all <m>z\in B_{r}(z_0)</m> we have 
                    <me>
                        \abs{f_k(z)-f(z)}\leq (r/R)^k\cdot \frac{MR}{R-r}&lt; \epsilon
                    </me>
                    for all <m>k\geq N</m>. This shows that <m>f_k\to f</m> uniformly on <m>B_r(z_0)</m>, as claimed.
                </p>
            </li>
        </ol>
    </p>
    </proof>
    </theorem>
    <corollary xml:id="cor_radius_convergence">
        <title>Radius of convergence</title>
        <statement>
            <p>
               Let <m>f(z)=\sum_{n=0}^\infty a_n (z-z_0)^n</m> be a complex power series. There is a unique extended real number <m>R\in [0,\infty)\cup \{\infty\}</m> satisfying the properties below. 
               <ol marker="(i)">
                <li>
                    <p>
                        <m>f</m> converges for all <m>z</m> satisfying <m>\abs{z-z_0}&lt; R</m>.
                    </p>
                </li>
                <li>
                    <p>
                        <m>f</m> diverges for all <m>z</m> satisfying <m>\abs{z-z_0}&gt; R</m>. 
                    </p>
                </li>
               </ol> 
            </p>
        </statement>
    </corollary>
    <definition xml:id="d_">
    <title>Radius of convergence</title>
    <statement>
    <p>
    The <term>radius of convergence</term> of a power series <m>f(z)=\sum_{n=0}^\infty a_nz^n</m> is the unique extended real number <m>R\in [0,\infty)\cup \{\infty\}</m> satisfying properties (i)-(ii) in <xref ref="cor_radius_convergence"/>. The <term>circle of convergence</term> of the power series <m>f</m> is the set <m>\{z\in \C\colon \abs{z-z_0}=R\}</m>. 
    </p>
    </statement>
    </definition>
    <theorem xml:id="th_power_series_integral_der">
    <title>Power series integration and differentiation</title>
    <statement>
    <p>
    Let <m>f(z)=\sum_{n=0}^\infty a_nz^n</m> be a power series with radius of convergence <m>R</m>. 
    <ol>
        <li>
            <p>
                <m>f</m> is continuous on <m>B_R(z_0)</m>. 
            </p>
        </li>
        <li>
            <p>
                <m>f</m> is holomorphic on <m>B_R(z_0)</m> and 
                <men xml:id="eq_power_series_der">
                f'(z)=a_1+2a_2z+3a_3z^2+\cdots=\sum_{n=0}^\infty (n+1)a_{n+1}z^n
                </men>. 
                In other words, we a power series representation of <m>f'</m> by differentiating <m>f</m> term by term. 
            </p>
        </li>
        <li>
            <p>
                For any path <m>\gamma</m> lying in <m>B_{R}(z_0)</m>, we have 
                <men xml:id="eq_power_series_int">
                    \int_\gamma f\, dz=\sum_{n=0}^\infty \int_\gamma a_n(z-z_0)\, dz
                </men>.
                
            </p>
        </li>
    </ol>
    </p>
    </statement>
    <proof>
    <p>
    </p>
    </proof>
    </theorem>
    <definition xml:id="d_analytic">
    <title>Analytic functions</title>
    <statement>
    <p>
    Let <m>f\colon U\rightarrow \C</m> be a complex function, with <m>U</m> an open set. We say <m>f</m> is <term>analytic at a point</term>  <m>z_0\in U</m> if <m>f</m> has a power series representation <m>f(z)=\sum_{n=0}^\infty a_n(z-z_0)^n</m> with positive radius of convergence. We say <m>f</m> is <term>analytic on a set</term> <m>D\subseteq U</m> if <m>f</m> is analytic at all points in <m>D</m>, and we say <m>f</m> is <term>analytic</term> if it is analytic on its domain.  
    </p>
    </statement>
    </definition>
    <corollary xml:id="cor_analytic_implies_holomorphic">
        <title>Analytic implies holomorphic</title>
        <statement>
            <p>
                Let <m>U\subseteq \C</m> be an open set.   If <m>f</m> is analytic on <m>U</m>, then <m>f</m> is holomorphic on <m>U</m>. Furthermore, for any <m>z_0\in U</m> we have power series representation <m>f(z)=\sum_{n=0}^\infty a_n(z-z_0)^n</m> with positive radius of convergence, where 
                <men>
                    a_n=\frac{1}{n!}f^{(n)}(z_0)=\frac{1}{2\pi i}\int_\gamma \frac{f(z)}{(z-z_0)^{n+1}}
                </men>,
                where <m>\gamma</m> is the counterclockwise oriented boundary of any closed disk <m>\overline{B}\subseteq U</m> containing <m>z_0</m>. 
            </p>
        </statement>
    </corollary>

    
    
    
    

</section>