<?xml version="1.0" encoding="UTF-8"?>

<section xml:id="s_sequences" xmlns:xi="http://www.w3.org/2001/XInclude">
    <title>Sequences and series</title>
    
    <introduction>
        <p>
        The complex modulus function <m>\abs{z}</m>, as well as the distance function <m>d(z,w)=\abs{z-w}</m> it defines, gives rise to theory of convergence of complex sequences and series that is a straightforward generalization of real sequences and series theory. 
        </p>
    </introduction>
<subsection xml:id="ss_sequences">
<title>Sequences</title>
<definition xml:id="d_lim_seq">
<title>Limit of sequence</title>
<statement>
<p>
A sequence of complex numbers <m>(z_n)_{n=1}^\infty=z_1,z_2,\dots</m> of complex numbers <term>converges</term> if there is a complex number <m>z\in \C</m> satisfying the following property: for all <m>\epsilon &gt; 0</m>, there exists a <m>N &gt; 0</m> such that if <m>n\geq N</m>, then <m>\abs{z_n-z}&lt; \epsilon</m>. 
We write <m>\lim\limits_{n\to \infty}z_n=z</m> (or <m>z_n\to z</m>) in this case, and call <m>z</m> the <term>limit</term> of the sequence. 
</p>
<p>
    A sequence <term>diverges</term> if it does not converge. 
</p>
</statement>
</definition>


<definition xml:id="d_lim_seq_inf">
<title>Infinite limit</title>
<statement>
<p>
A complex sequence <m>(z_n)_{n=1}^\infty</m> has an <term>infinite limit</term>, denoted <m>\lim\limits_{n\to \infty}z_n=\infty</m> if for all <m>R&gt; 0</m>, there exists an <m>N&gt; 0</m> such that if <m>n\geq N</m>, then <m>\abs{z_n}&gt; R</m>. 
</p>
</statement>
</definition>
<remark>
<title>Infinite limit</title>
<p>
Identifying an element <m>z</m> of <m>\C^*=\C\cup \{\infty\}</m> with its corresponding point <m>P_z\in S^2\subseteq \R^3</m> using the stereographic projection, you can show that 
<md>
    <mrow>z_n\to \infty \amp \iff P_{z_n}\to N=(0,0,1)</mrow>
</md>. 
</p>
</remark>

<remark>
<title>Logical shorthand</title>
<p>
<xref first="d_lim_seq" last="d_lim_seq_inf"/>, can be expressed using logical shorthand as follows: 
<mdn>
    <mrow>z_n\to z \amp \iff \forall \epsilon &gt; 0\, \exists N &gt; 0( n\geq N \implies \abs{z_n-z}&lt; \epsilon) </mrow>
    <mrow>z_n\to\infty \amp \iff \forall R &gt; 0\, \exists N &gt; 0( n\geq N \implies \abs{z_n}&gt; R) </mrow>
</mdn>.
</p>
</remark>
<p>
  Limits of complex sequences satisfy all the usual familiar limit properties of real sequences, and then some.   
</p>
<theorem xml:id="th_lim">
<title>Limit properties</title>
<statement>
<p>
    Let <m>(z_n)_{n=1}^\infty</m> and <m>(w_n)_{n=1}^\infty</m> be sequences of complex numbers. 
<ol>
   <li>
      <p>
         <m>z_{n}\rightarrow z</m> if and only if <m>\val{z_n-z}\rightarrow 0</m>. 
      </p>
      <p>
        In particular, <m>z_{n}\rightarrow 0</m> if and only if <m>\val{z_n}\rightarrow 0</m>.
      </p>
   </li>

   <li>
      <p>
         <m>\{z_{n}\}</m> converges if and only if <m>\{\Re z_{n}\}</m> and <m>\{\Im z_{n}\}</m> both converge, in which case 
         <md>
         <mrow> \lim_{n\rightarrow\infty}z_{n}\amp = (\lim_{n\rightarrow\infty}\Re z_{n})+i\lim\limits_{n\to \infty}\Im z_n </mrow>
         </md>.
         In particular, we have <m>\lim\limits_{n\to \infty}z_n=z</m> if and only if 
            <md>
                <mrow>\lim\limits_{n\to \infty}\Re z_n \amp =\Re z \amp 
                \lim\limits_{n\to \infty}\Im z_n= \Im z</mrow>
            </md>.
      </p>
   </li>
    <li>
        <p>
            <m>z_n\to z</m> if and only if <m>\overline{z_n}\to \overline{z}</m>. 
        </p>
    </li>
   <li>
      <p>
         If <m>z_{n}\rightarrow z</m>, then <m>\val{z_n}\rightarrow \val{z}</m>.
      </p>
   </li>

   <li>
      <p>
         If <m>\lim\limits_{n\to \infty}z_n=z</m> and <m>\lim\limits_{n\to \infty}w_n=w</m>, then
         <mdn>
            <mrow xml:id="eq_lim_seq_linear">\lim\limits_{n\to \infty} cz_{n}+\lim\limits_{n\to \infty}dw_{n}\amp = c\lim\limits_{n\to \infty}z_n+d\lim\limits_{n\to \infty}w_n=cz+dw \text{ for any } c,d\in \C</mrow>
            <mrow> \lim\limits_{n\to \infty}z_{n}w_{n}\amp = (\lim\limits_{n\to \infty}z_n)(\lim\limits_{n\to \infty}w_m)=zw\amp </mrow>
            <mrow> \lim\limits_{n\to \infty}\frac{z_n}{w_n}\amp = \frac{\lim\limits_{n\to \infty}z_n}{\lim\limits_{n\to \infty}w_n}= z/w,  \text{ assuming } w\ne 0 </mrow>
         </mdn>.
      </p>
   </li>
   

   <li>
      <p>
         <m>z_{n}\rightarrow \infty</m> if and only if <m>\frac{1}{z_{n}}\rightarrow 0</m>, assuming <m>z_n\ne 0</m> for all <m>n</m>. 
      </p>
   </li>
</ol>
</p>
</statement>
<proof>
<p>
    Most of these statements are proved exactly as with their analogous statements for real sequences, and both in turn use little beyond properties of <m>\abs{\ }</m>, either as the absolute value (on the reals) or its extension, the complex modulus. We content ourselves with proving (2) by way of illustration. 
</p>
<p>
    For the reverse direction (<m>\Leftarrow</m>), if both <m>\lim\limits_{n\to \infty}\Re z_n</m> and <m>\lim\limits_{n\to \infty}\Im z_n</m> exist, then we have 
    <md>
        <mrow>\lim\limits_{n\to \infty}z_n\amp = \lim\limits_{n\to \infty}\Re z_n+i\Im z_n \amp </mrow>
        <mrow> \amp =\lim\limits_{n\to \infty}\Re z_n+i\lim\limits_{n\to \infty}\Im z_n \amp (<xref ref="eq_lim_seq_linear"/>) </mrow>
    </md>,
    as desired.
</p>
<p>
    Consider now the forward implication (<m>\Rightarrow</m>). We assume <m>\lim\limits_{n\to \infty}z_n=z</m> and wish to show that <m>\Re z=\lim\limits_{n\to \infty}\Re z_n</m> and  <m>\Im z=\lim\limits_{n\to \infty}\Im z_n</m> (which also proves these limits exists). We will give a proof of the second equality: you can prove the first in much the same way. Fix any positive <m>\epsilon &gt; 0</m>. Since <m>z_n\rightarrow z</m>, we can find an <m>N&gt; 0</m> such that <m>\abs{z-z_n}&lt; \epsilon</m> for all <m>n\geq N</m>. But then we have 
    <md>
        <mrow>\abs{\Im z-\Im z_n} \amp =\abs{\Im(z-z_n)}</mrow>
        <mrow> \amp \leq \abs{z-z_n} </mrow>
        <mrow> \amp &lt; \epsilon</mrow>
    </md>
    for all <m>n\geq N</m>, showing that <m>\Im z_n\to \Im z</m>, as desired. 
</p>
</proof>
</theorem>
<example xml:id="eg_lim_seq">
<title>Limit of sequence</title>
<statement>
<p>
Define <m>z_n=\frac{1}{2^n}(1+i)^n</m>. Show that <m>(z_n)_{n=1}^{\infty}</m> converges and compute its limit. 
</p>
</statement>
<solution>
<p>
We have <m>z_n=w^n</m>, where <m>w=\frac{1}{2}(1+i)=\frac{\sqrt{2}}{2}(\cos(\pi/4)+i\sin(\pi/4))</m>. It follows from de Moivre's formula that 
<me>
z_n=w^n=(\sqrt{2}/2)^n(\cos(n\pi/4)+i\sin(n\pi/4))
</me>
and hence that 
<me>
\abs{z_n}=(\sqrt{2}/2)^n.
</me>
Since <m>(\sqrt{2}/2)&lt; 1</m>, we have <m>\abs{z_n}\to 0</m>. It follows from <xref ref="th_lim"/> that <m>z_n\to 0</m>. 
</p>
</solution>
</example>
<example xml:id="eg_lim_seq_div">
<title>Divergent sequence</title>
<statement>
<p>
Show that the sequence <m>(i^n)_{n=1}^{\infty}</m> diverges. 
</p>
</statement>
<solution>
<p>
Observe first that the sequence is periodic of the form 
\[
i,-1,-i,1,i,-1,\dots
\]
Assume by contradiction that <m>i^n\to w</m> for some complex number <m>w</m>. Taking <m>\epsilon =1</m> in the definition of sequence convergence, this would imply the existence of an <m>N</m> such that <m>\abs{i^n-w}&lt; 1</m> for all <m>n\geq N</m>. In particular, we would have  <m>\abs{1-w}&lt; 1</m> and <m>\abs{-1-w}&lt; 1</m>. But this would imply that 
<md>
    <mrow>2=\abs{1+1} \amp = \abs{1-w-(-1-w)} </mrow>
    <mrow> \amp\leq \abs{1-w}+\abs{-1-w} </mrow>
    <mrow> \amp &lt; 1+1=2</mrow>
</md>,
a contradiction since then we'd have <m>2&lt; 2</m>. We conclude that there is no limit to the sequence. 
</p>
</solution>
</example>
<example xml:id="eg_lim_seq_inf">
<title>Sequence with infinite limit</title>
<statement>
<p>
Show that <m>\lim\limits_{n\to \infty}\frac{\sqrt{n}i+n^2}{5n+i}=\infty</m>. 
</p>
</statement>
<solution>
<p>
Let <m>z_n=\frac{\sqrt{n}i+n^2}{5n+i}</m>. 
We will show that <m>\frac{1}{z_n}\to 0</m>, and thus <m>z_n\to \infty</m>, by <xref ref="th_lim"/>.  Looking at 
<me>
    \frac{1}{z_n}=\frac{5n+i}{\sqrt{n}i+n^2}
</me>
we see that the dominating term on top is the <m>5n</m> and the dominating term on the bottom is <m>n^2</m>. We will make this argument rigorous by factoring out these dominating terms from the top and bottom and computing the limit 
using a combination of algebra and limit rules.
<md>
    <mrow> \lim\limits_{n\to \infty}\frac{1}{z_n}\amp= \lim\limits_{n\to \infty}\frac{5n+i}{\sqrt{n}i+n^2} </mrow>
    <mrow> \amp = \lim\limits_{n\to \infty}\frac{n\left(5+\frac{i}{n}\right)}{n^2\left(\frac{i}{n^{3/2}}+1\right)} </mrow>
    <mrow> \amp = \lim\limits_{n\to \infty}\frac{1}{n} \cdot \frac{5+\frac{i}{n}}{\frac{i}{n^{3/2}}+1}</mrow>
    <mrow> \amp = \lim\limits_{n\to \infty}\frac{1}{n} \cdot \lim\limits_{n\to \infty}\frac{5+\frac{i}{n}}{\frac{i}{n^{3/2}}+1} \amp (\text{prod. rule})</mrow>
    <mrow> \amp =\lim\limits_{n\to \infty}\frac{1}{n}\cdot  \frac{5+i\lim\limits_{n\to \infty}\frac{1}{n}}{i\lim\limits_{n\to \infty}\frac{1}{n^{3/2}}+1} \amp (\text{quot., sum, scal. rule})
    \amp (n\to 0) </mrow>
    <mrow> \amp =0\cdot \frac{5}{1}</mrow>
    <mrow> \amp =0 </mrow>
</md>.
Since <m>1/z_n\to 0</m>, we conclude that <m>z_n\to \infty</m>. 
</p>
</solution>
</example>


</subsection>
<subsection xml:id="ss_series">
<title>Series</title>
<p>
    As with the reals, from a theory of convergent <em>sequences</em> we easily derive a theory of convergent <em>series</em>. The definitions and results below are all straightforward generalizations of facts about series of real numbers. 
</p>
<definition xml:id="d_series">
<title>Series</title>
<statement>
<p>
Given a complex sequence <m>(z_n)_{n=1}^{\infty}</m>, the formal expression <m>\sum_{n=1}^\infty z_n</m> is called a <term>(complex) series</term>. 
</p>
<p>
    For each <m>k\geq 1</m> we define the <term><m>k</m>-th partial sum</term> <m>S_k</m> of the series <m>\sum_{n=1}^\infty z_n</m> as 
    <me>
        S_k=\sum_{n=1}^k z_k
    </me>.
  We say the series <term>converges</term> if 
  <me>
    \lim\limits_{k\to \infty}S_k=\lim\limits_{k\to \infty}\sum_{n=1}^k z_k=z
  </me>
    for some complex number <m>z\in \C</m>, in which case we write 
    <me>
        \sum_{n=1}^\infty z_n=z
    </me>
    and say that the series converges to <m>z</m>. 
</p>
    <p>
        A series <term>diverges</term> if it does not converge. 
    </p>
</statement>
</definition>


<theorem xml:id="th_series">
<title>Series properties</title>
<statement>
<p>
Let <m>(z_n)_{n=1}^\infty</m> and <m>(w_n)_{n=1}^\infty</m> be complex sequences.
<ol>
    <li>
        <p>
            <m>\sum_{n=1}^\infty z_n=z</m> if and only if <m>\lim\limits_{k\to \infty}(S_k-z)=0</m>, where <m>S_k</m> is the <m>k</m>-th partial sum of <m>\sum_{n=1}^\infty z_n</m>. 
        </p>
    </li>
    <li>
        <p>
            <m>\sum_{n=1}^\infty z_n</m> converges if and only if <m>\sum_{n=1}^\infty \Re z_n</m> and <m>\sum_{n=1}^\infty \Im z_n</m> converge, in which case
            <me>
                \sum_{n=1}^\infty z_n=\sum_{n=1}^\infty \Re z_n +i \sum_{n=1}^\infty \Im z_n
            </me>.
           In particular, <m>\sum_{n=1}^\infty z_n=z</m> if and only if 
           <md>
            <mrow>\sum_{n=1}^\infty \Re z_n \amp = \Re z \amp \sum_{n=1}^\infty \Im z_n=\Im z</mrow>
           </md> 
        </p>
    </li>
    <li>
        <p>
            If <m>\sum_{n=1}^\infty z_n=z</m> and <m>\sum_{n=1}^\infty w_n=w</m>, then 
            <md>
                <mrow> \sum_{n=1}^\infty cz_n+\sum_{n=1}^\infty dw_n \amp = c\sum_{n=1}^\infty z_n+d\sum_{n=1}^\infty w_n  </mrow>
                <mrow> \amp =cz+dw </mrow>
            </md>,
            for any <m>c,w\in \C</m>. 
        </p>
    </li>
    <li>
    <title>Divergence test</title>
    <p>
        If <m>\sum_{n=1}^\infty z_n</m> converges, then <m>\lim\limits_{n\to \infty}z_n=0</m>.
    </p>
   </li>
   <li>
    <title>Absolute convergence test</title>
    <p>
        If <m>\sum_{n=1}^\infty \abs{z_n}</m> converges, then <m>\sum_{n=1}^\infty z_n</m> converges and 
        <me>
            \abs{\sum_{n=1}^\infty z_n}\leq \sum_{n=1}^\infty \abs{z_n}
        </me>.
    </p>
   </li>
</ol> 
</p>
</statement>
<proof>
<p>
</p>
</proof>
</theorem>
<example xml:id="eg_geom_series">
<title>Geometric series</title>
<statement>
<p>
Let <m>z\in \C</m>. Show that the <term>geometric series</term> <m>\sum_{n=0}^\infty z^n</m> converges to <m>\frac{1}{1-z}</m> if <m>\abs{z}&lt; 1</m>, and diverges for <m>\abs{z}\geq 1</m>. 
</p>
</statement>
<solution>
<p>
First observe that if <m>\abs{z}\geq 1</m>, then the sequence <m>(\abs{z^n})\not\to 0</m>. It follows that <m>z_n\not\to 0</m> and thus that the series diverges by the divergence test. 
</p>
<p>
    Now assume <m>\abs{z}&lt; 1</m>. For all <m>k\geq 1</m> the <m>k</m>-th partia sum is 
    <me>
        S_k=1+z+z^2+\cdots + z^k=\frac{z^{k+1}-1}{z-1},
    </me>
    using the polynomial identity <xref ref="eq_cyclo_factor"/>. It follows that 
    <md>
        <mrow>\sum_{n=0}^\infty z^n \amp =\lim_{k\to\infty}S_k</mrow>
        <mrow> \amp =\lim_{k\to\infty}\frac{z^{k+1}-1}{z-1}</mrow>
        <mrow> \amp =\frac{\lim_{k\to\infty}z^{k+1}-1}{\lim_{k\to\infty}z-1}</mrow>
        <mrow> \amp =\frac{0-1}{z-1} \amp (\abs{z}&lt; 0\implies z^{k+1}\to 0)</mrow>
        <mrow> \amp =\frac{1}{1-z}</mrow>
    </md>.
</p>
</solution>
</example>

</subsection>
</section>